proof/refine/ARM_HYP/ArchCSpace_R.thy
@@ -437,10 +437,12 @@ lemma corres_caps_decomposition:
                    g \<lbrace>\<lambda>rv s. P (ksReadyQueues s) (tcbSchedNexts_of s) (tcbSchedPrevs_of s)
                                (\<lambda>d p. inQ d p |< tcbs_of' s)\<rbrace>"
              "\<And>P. \<lbrace>\<lambda>s. P (new_di s)\<rbrace> f \<lbrace>\<lambda>rv s. P (domain_index s)\<rbrace>"
+             "\<And>P. \<lbrace>\<lambda>s. P (new_ds s)\<rbrace> f \<lbrace>\<lambda>rv s. P (domain_start_index s)\<rbrace>"
              "\<And>P. \<lbrace>\<lambda>s. P (new_dl s)\<rbrace> f \<lbrace>\<lambda>rv s. P (domain_list s)\<rbrace>"
              "\<And>P. \<lbrace>\<lambda>s. P (new_cd s)\<rbrace> f \<lbrace>\<lambda>rv s. P (cur_domain s)\<rbrace>"
              "\<And>P. \<lbrace>\<lambda>s. P (new_dt s)\<rbrace> f \<lbrace>\<lambda>rv s. P (domain_time s)\<rbrace>"
              "\<And>P. \<lbrace>\<lambda>s. P (new_dsi' s)\<rbrace> g \<lbrace>\<lambda>rv s. P (ksDomScheduleIdx s)\<rbrace>"
+             "\<And>P. \<lbrace>\<lambda>s. P (new_dss' s)\<rbrace> g \<lbrace>\<lambda>rv s. P (ksDomScheduleStart s)\<rbrace>"
              "\<And>P. \<lbrace>\<lambda>s. P (new_ds' s)\<rbrace> g \<lbrace>\<lambda>rv s. P (ksDomSchedule s)\<rbrace>"
              "\<And>P. \<lbrace>\<lambda>s. P (new_cd' s)\<rbrace> g \<lbrace>\<lambda>rv s. P (ksCurDomain s)\<rbrace>"
              "\<And>P. \<lbrace>\<lambda>s. P (new_dt' s)\<rbrace> g \<lbrace>\<lambda>rv s. P (ksDomainTime s)\<rbrace>"
@@ -459,8 +461,11 @@ lemma corres_caps_decomposition:
                   \<and> new_id s = new_id' s'
                   \<and> new_ms s = new_ms' s'
                   \<and> new_di s = new_dsi' s'
-                  \<and> new_dl s = new_ds' s'
-                  \<and> new_cd s = new_cd' s'
+                  \<and> new_ds s = new_dss' s'
+                            \<and> domain_list_map (new_dl s) = new_ds' s'
+
+
+                            \<and> new_cd s = new_cd' s'
                   \<and> new_dt s = new_dt' s'
                   \<and> new_wuc s = new_wuc' s'
                   \<and> new_ups s = new_ups' s'
@@ -705,7 +710,7 @@ lemma setupReplyMaster_invs'[wp]:
    apply (wpsimp wp: setupReplyMaster_valid_pspace' sch_act_wf_lift tcb_in_cur_domain'_lift
                      ct_idle_or_in_cur_domain'_lift
                      valid_queues_lift cur_tcb_lift hoare_vcg_disj_lift sym_heap_sched_pointers_lift
-                     valid_bitmaps_lift valid_irq_node_lift
+                     valid_bitmaps_lift valid_irq_node_lift valid_dom_schedule'_lift
           | rule refl)+
   apply (clarsimp simp: ex_nonz_tcb_cte_caps' valid_pspace'_def
                         gen_objBits_simps tcbReplySlot_def
