proof/refine/CSpace_R.thy
@@ -793,14 +793,15 @@ lemma next_slot_eq2:
 lemma set_cap_not_quite_corres':
   assumes cr:
   "pspace_relation (kheap s) (ksPSpace s')"
-  "cur_thread s    = ksCurThread s'"
-  "idle_thread s   = ksIdleThread s'"
+  "cur_thread s = ksCurThread s'"
+  "idle_thread s = ksIdleThread s'"
   "machine_state s = ksMachineState s'"
   "work_units_completed s = ksWorkUnitsCompleted s'"
-  "domain_index s  = ksDomScheduleIdx s'"
-  "domain_list s   = ksDomSchedule s'"
-  "cur_domain s    = ksCurDomain s'"
-  "domain_time s   = ksDomainTime s'"
+  "domain_index s = ksDomScheduleIdx s'"
+  "domain_start_index s = ksDomScheduleStart s'"
+  "domain_list_map (domain_list s) = ksDomSchedule s'"
+  "cur_domain s = ksCurDomain s'"
+  "domain_time s = ksDomainTime s'"
   "(x,t') \<in> fst (updateCap p' c' s')"
   "valid_objs s" "pspace_aligned s" "pspace_distinct s" "cte_at p s"
   "pspace_aligned' s'" "pspace_distinct' s'"
@@ -810,22 +811,23 @@ lemma set_cap_not_quite_corres':
   assumes p: "p' = cte_map p"
   shows "\<exists>t. ((),t) \<in> fst (set_cap c p s) \<and>
              pspace_relation (kheap t) (ksPSpace t') \<and>
-             cdt t              = cdt s \<and>
-             cdt_list t         = cdt_list (s) \<and>
+             cdt t = cdt s \<and>
+             cdt_list t = cdt_list (s) \<and>
              scheduler_action t = scheduler_action (s) \<and>
-             ready_queues t     = ready_queues (s) \<and>
-             is_original_cap t  = is_original_cap s \<and>
+             ready_queues t = ready_queues (s) \<and>
+             is_original_cap t = is_original_cap s \<and>
              interrupt_state_relation (interrupt_irq_node t) (interrupt_states t)
-                              (ksInterruptState t') \<and>
+                                      (ksInterruptState t') \<and>
              (arch_state t, ksArchState t') \<in> arch_state_relation \<and>
-             cur_thread t    = ksCurThread t' \<and>
-             idle_thread t   = ksIdleThread t' \<and>
+             cur_thread t = ksCurThread t' \<and>
+             idle_thread t = ksIdleThread t' \<and>
              machine_state t = ksMachineState t' \<and>
              work_units_completed t = ksWorkUnitsCompleted t' \<and>
-             domain_index t  = ksDomScheduleIdx t' \<and>
-             domain_list t   = ksDomSchedule t' \<and>
-             cur_domain t    = ksCurDomain t' \<and>
-             domain_time t   = ksDomainTime t'"
+             domain_index t = ksDomScheduleIdx t' \<and>
+             domain_start_index t  = ksDomScheduleStart t' \<and>
+             domain_list_map (domain_list t) = ksDomSchedule t' \<and>
+             cur_domain t = ksCurDomain t' \<and>
+             domain_time t = ksDomainTime t'"
   using cr
   by (rule set_cap_not_quite_corres; fastforce simp: c p)
 
@@ -1011,7 +1013,7 @@ lemma cteMove_corres:
   apply (clarsimp simp: split_def)
   apply (rule bind_execI, assumption)
   apply (drule_tac p=ptr and c="cap.NullCap" in set_cap_not_quite_corres')
-                 apply assumption+
+                      apply (assumption | solves \<open>simp add: split_def\<close>)+
             apply (frule use_valid [OF _ set_cap_valid_objs])
              apply fastforce
             apply assumption
@@ -1074,7 +1076,7 @@ lemma cteMove_corres:
   apply (subgoal_tac "\<forall>p. cte_at p ta = cte_at p a")
    prefer 2
    apply (simp add: set_cap_cte_eq)
-  apply (clarsimp simp add: swp_def cte_wp_at_ctes_of simp del: split_paired_All)
+  apply (clarsimp simp add: swp_def cte_wp_at_ctes_of split_def simp del: split_paired_All)
   apply (subgoal_tac "cte_at ptr' a")
    prefer 2
    apply (erule cte_wp_at_weakenE, rule TrueI)
@@ -1090,6 +1092,7 @@ lemma cteMove_corres:
   apply (thin_tac "ksWorkUnitsCompleted t = p" for t p)+
   apply (thin_tac "cur_thread t = p" for t p)+
   apply (thin_tac "domain_index t = p" for t p)+
+  apply (thin_tac "domain_start_index t = p" for t p)+
   apply (thin_tac "domain_time t = p" for t p)+
   apply (thin_tac "cur_domain t = p" for t p)+
   apply (thin_tac "scheduler_action t = p" for t p)+
@@ -1102,6 +1105,7 @@ lemma cteMove_corres:
   apply (thin_tac "ksCurDomain t = p" for t p)+
   apply (thin_tac "ksInterruptState t = p" for t p)+
   apply (thin_tac "ksDomScheduleIdx t = p" for t p)+
+  apply (thin_tac "ksDomScheduleStart t = p" for t p)+
   apply (thin_tac "ksDomainTime t = p" for t p)+
   apply (thin_tac "ksDomSchedule t = p" for t p)+
   apply (thin_tac "pspace_relation t p" for t p)+
@@ -3057,73 +3061,25 @@ lemma setCTE_ct_not_inQ[wp]:
        apply (clarsimp simp add: obj_at'_def)+
   done
 
-crunch cteInsert
+crunch setCTE, cteInsert
   for ct_not_inQ[wp]: "ct_not_inQ"
-  (simp: crunch_simps wp: hoare_drop_imp)
-
-lemma setCTE_ksCurDomain[wp]:
-  "\<lbrace>\<lambda>s. P (ksCurDomain s)\<rbrace>
-   setCTE p cte
-   \<lbrace>\<lambda>rv s. P (ksCurDomain s)\<rbrace>"
-  apply (simp add: setCTE_def)
-  apply wp
-  done
-
-lemma setObject_cte_ksDomSchedule[wp]: "\<lbrace> \<lambda>s. P (ksDomSchedule s) \<rbrace> setObject ptr (v::cte) \<lbrace> \<lambda>_ s. P (ksDomSchedule s) \<rbrace>"
-  apply (simp add: setObject_def split_def)
-  apply (wp updateObject_cte_inv | simp)+
-  done
-
-lemma setCTE_ksDomSchedule[wp]:
-  "\<lbrace>\<lambda>s. P (ksDomSchedule s)\<rbrace>
-   setCTE p cte
-   \<lbrace>\<lambda>rv s. P (ksDomSchedule s)\<rbrace>"
-  apply (simp add: setCTE_def)
-  apply wp
-  done
-
-crunch cteInsert
-  for ksCurDomain[wp]: "\<lambda>s. P (ksCurDomain s)"
-  (wp:  crunch_wps )
-
-crunch cteInsert
-  for ksIdleThread[wp]: "\<lambda>s. P (ksIdleThread s)"
-  (wp: crunch_wps)
-
-crunch cteInsert
-  for ksDomSchedule[wp]: "\<lambda>s. P (ksDomSchedule s)"
-  (wp: crunch_wps)
-
-lemma setCTE_tcbDomain_inv[wp]:
-  "\<lbrace>obj_at' (\<lambda>tcb. P (tcbDomain tcb)) t\<rbrace> setCTE ptr v \<lbrace>\<lambda>_. obj_at' (\<lambda>tcb. P (tcbDomain tcb)) t\<rbrace>"
-  by (simp add: setCTE_def)
-     (rule setObject_cte_obj_at_tcb', simp_all)
+  and ksCurDomain[wp]: "\<lambda>s. P (ksCurDomain s)"
+  and ksIdleThread[wp]: "\<lambda>s. P (ksIdleThread s)"
+  and ksDomSchedule[wp]: "\<lambda>s. P (ksDomSchedule s)"
+  and ksDomScheduleIdx[wp]: "\<lambda>s. P (ksDomScheduleIdx s)"
+  and ksDomScheduleStart[wp]: "\<lambda>s. P (ksDomScheduleStart s)"
+  (wp: updateObject_cte_inv crunch_wps simp: setObject_def)
 
 crunch cteInsert
   for tcbDomain_inv[wp]: "obj_at' (\<lambda>tcb. P (tcbDomain tcb)) t"
-  (wp: crunch_simps hoare_drop_imps)
-
-lemma setCTE_tcbPriority_inv[wp]:
-  "setCTE ptr v \<lbrace> obj_at' (\<lambda>tcb. P (tcbPriority tcb)) t\<rbrace>"
-  by (auto simp: setCTE_def intro: setObject_cte_obj_at_tcb')
-
-crunch cteInsert
-  for tcbPriority_inv[wp]: "obj_at' (\<lambda>tcb. P (tcbPriority tcb)) t"
-  (wp: crunch_simps hoare_drop_imps)
+  and tcbPriority_inv[wp]: "obj_at' (\<lambda>tcb. P (tcbPriority tcb)) t"
+  (wp: crunch_simps hoare_drop_imps setObject_cte_obj_at_tcb')
 
 lemma cteInsert_ct_idle_or_in_cur_domain'[wp]:
   "\<lbrace> ct_idle_or_in_cur_domain' \<rbrace> cteInsert a b c \<lbrace> \<lambda>_. ct_idle_or_in_cur_domain' \<rbrace>"
   apply (rule ct_idle_or_in_cur_domain'_lift)
   apply (wp hoare_vcg_disj_lift)+
   done
-
-lemma setObject_cte_domIdx:
-  "\<lbrace>\<lambda>s. P (ksDomScheduleIdx s)\<rbrace> setObject t (v::cte) \<lbrace>\<lambda>rv s. P (ksDomScheduleIdx s)\<rbrace>"
-  by (clarsimp simp: valid_def setCTE_def[symmetric] dest!: setCTE_pspace_only)
-
-crunch cteInsert
-  for ksDomScheduleIdx[wp]: "\<lambda>s. P (ksDomScheduleIdx s)"
-  (wp: setObject_cte_domIdx hoare_drop_imps)
 
 crunch cteInsert
   for gsUntypedZeroRanges[wp]: "\<lambda>s. P (gsUntypedZeroRanges s)"
@@ -3292,7 +3248,7 @@ lemma cteInsert_invs:
   apply (simp add: invs'_def valid_state'_def valid_pspace'_def)
   apply (wpsimp wp: cur_tcb_lift tcb_in_cur_domain'_lift sch_act_wf_lift
                     valid_irq_node_lift irqs_masked_lift cteInsert_norq
-                    sym_heap_sched_pointers_lift)
+                    sym_heap_sched_pointers_lift valid_dom_schedule'_lift)
   apply (auto simp: invs'_def valid_state'_def valid_pspace'_def elim: valid_capAligned)
   done
 
@@ -3868,6 +3824,7 @@ crunch setupReplyMaster
   and ct_not_inQ[wp]: "ct_not_inQ"
   and ksCurDomain[wp]: "\<lambda>s. P (ksCurDomain s)"
   and ksDomSchedule[wp]: "\<lambda>s. P (ksDomSchedule s)"
+  and ksDomScheduleStart[wp]: "\<lambda>s. P (ksDomScheduleStart s)"
   and tcbDomain_inv[wp]: "obj_at' (\<lambda>tcb. P (tcbDomain tcb)) t"
   and tcbPriority_inv[wp]: "obj_at' (\<lambda>tcb. P (tcbPriority tcb)) t"
   and ready_queuesL1[wp]: "\<lambda>s. P (ksReadyQueuesL1Bitmap s)"
@@ -4023,7 +3980,7 @@ lemma arch_update_setCTE_invs:
             arch_update_setCTE_iflive arch_update_setCTE_ifunsafe
             valid_irq_node_lift setCTE_typ_at' setCTE_irq_handlers' irqs_masked_lift
             hoare_vcg_disj_lift untyped_ranges_zero_lift valid_bitmaps_lift
-            setCTE_valid_arch
+            setCTE_valid_arch valid_dom_schedule'_lift
            | simp add: pred_tcb_at'_def)+
   apply (clarsimp simp: valid_global_refs'_def is_arch_update'_def fun_upd_def[symmetric]
                         cte_wp_at_ctes_of gen_isCap_simps untyped_ranges_zero_fun_upd)
@@ -4226,7 +4183,7 @@ lemma (in CSpace_R_2) cteInsert_simple_corres:
                apply (simp+)[3]
             apply (clarsimp simp: corres_underlying_def state_relation_def
                                   in_monad valid_mdb'_def valid_mdb_ctes_def)
-            apply (drule (18) set_cap_not_quite_corres)
+            apply (drule (19) set_cap_not_quite_corres)
              apply (rule refl)
             apply (elim conjE exE)
             apply (rule bind_execI, assumption)
@@ -4264,6 +4221,7 @@ lemma (in CSpace_R_2) cteInsert_simple_corres:
             apply (thin_tac "ksSchedulerAction t = p" for t p)+
             apply (thin_tac "cur_thread t = p" for t p)+
             apply (thin_tac "domain_index t = p" for t p)+
+            apply (thin_tac "domain_start_index t = p" for t p)+
             apply (thin_tac "domain_time t = p" for t p)+
             apply (thin_tac "cur_domain t = p" for t p)+
             apply (thin_tac "scheduler_action t = p" for t p)+
@@ -4276,6 +4234,7 @@ lemma (in CSpace_R_2) cteInsert_simple_corres:
             apply (thin_tac "ksCurDomain t = p" for t p)+
             apply (thin_tac "ksInterruptState t = p" for t p)+
             apply (thin_tac "ksDomScheduleIdx t = p" for t p)+
+            apply (thin_tac "ksDomScheduleStart t = p" for t p)+
             apply (thin_tac "ksDomainTime t = p" for t p)+
             apply (thin_tac "ksDomSchedule t = p" for t p)+
             apply (thin_tac "ctes_of t = p" for t p)+
@@ -5216,8 +5175,9 @@ lemma cteInsert_simple_invs:
    apply (simp add: invs'_def valid_state'_def valid_pspace'_def)
    apply (wp cur_tcb_lift sch_act_wf_lift valid_queues_lift tcb_in_cur_domain'_lift
              valid_irq_node_lift irqs_masked_lift sym_heap_sched_pointers_lift
-             cteInsert_simple_mdb' cteInsert_valid_globals_simple
-             cteInsert_norq | simp add: pred_tcb_at'_def)+
+             valid_dom_schedule'_lift
+             cteInsert_simple_mdb' cteInsert_valid_globals_simple cteInsert_norq
+          | simp add: pred_tcb_at'_def)+
   apply (auto simp: invs'_def valid_state'_def valid_pspace'_def
                     untyped_derived_eq_def o_def
               dest!: is_simple_cap'_genD
@@ -5366,7 +5326,7 @@ lemma updateFreeIndex_forward_invs':
       apply (simp add:updateCap_def)
       apply (wp irqs_masked_lift cur_tcb_lift ct_idle_or_in_cur_domain'_lift
                 hoare_vcg_disj_lift untyped_ranges_zero_lift getCTE_wp
-                sym_heap_sched_pointers_lift valid_bitmaps_lift
+                sym_heap_sched_pointers_lift valid_bitmaps_lift valid_dom_schedule'_lift
                | wp (once) hoare_use_eq[where f="gsUntypedZeroRanges"]
                | simp add: getSlotCap_def)+
   apply (clarsimp simp: cte_wp_at_ctes_of fun_upd_def[symmetric])
